Organized typing file

DeBruijnSSA/SingleApp/Typing.lean
@@ -4,9 +4,11 @@ import DeBruijnSSA.InstSet
 
 namespace SingleApp
 
+section Basic
+
 variable [Φ: InstSet φ (Ty α) ε] [PartialOrder α] [PartialOrder ε] [Zero ε]
 
-  inductive Ty (α : Type u) where
+inductive Ty (α : Type u) where
   | base : α → Ty α
   | pair : Ty α → Ty α → Ty α
   | unit : Ty α
@@ -53,6 +55,107 @@ structure Ctx.Var (Γ : Ctx α ε) (n : ℕ) (V : Ty α × ε) : Prop where
   length : n < Γ.length
   get : Γ.get ⟨n, length⟩ ≤ V
 
+instance : Append (Ctx α ε) := (inferInstance : Append (List (Ty α × ε)))
+
+def FCtx (α ε) := Σn, Fin n → Ty α × ε
+
+-- TODO: FCtx append
+
+inductive Term.Wf : Ctx α ε → Term φ → Ty α → ε → Prop
+  | var : Γ.Var n ⟨A, e⟩ → Wf Γ (var n) A e
+  | op : Φ.Fn f A B e → Wf Γ a A e → Wf Γ (op f a) B e
+  | pair : Wf Γ a A e → Wf Γ b B e → Wf Γ (pair a b) (Ty.pair A B) e
+  | unit (e) : Wf Γ unit Ty.unit e
+  | bool (b e) : Wf Γ (bool b) Ty.bool e
+
+inductive Term.WfD : Ctx α ε → Term φ → Ty α → ε → Type _
+  | var : Γ.Var n ⟨A, e⟩ → WfD Γ (var n) A e
+  | op : Φ.Fn f A B e → WfD Γ a A e → WfD Γ (op f a) B e
+  | pair : WfD Γ a A e → WfD Γ b B e → WfD Γ (pair a b) (Ty.pair A B) e
+  | unit (e) : WfD Γ unit Ty.unit e
+  | bool (b e) : WfD Γ (bool b) Ty.bool e
+
+def Term.min_ty (Γ : Ctx α ε) : Term φ → Ty α
+  | var n => if h : n < Γ.length then (Γ.get ⟨n, h⟩).1 else Ty.unit
+  | op f _ => Φ.trg f
+  | pair a b => Ty.pair (a.min_ty Γ) (b.min_ty Γ)
+  | unit => Ty.unit
+  | bool _ => Ty.bool
+
+-- TODO: WfD ==> Wf
+
+-- TODO: Wf ==> ∃WfD
+
+-- def Term.Wf.toWFD
+--   {Γ : Ctx α ε} {a : Term φ} {A e} (h : Wf Γ a A e) : WfD Γ a A e
+--   := match a with
+--   | Term.var n => WfD.var sorry
+--   | Term.op f a => WfD.op sorry sorry
+--   | Term.pair a b => WfD.pair sorry sorry
+--   | Term.unit => sorry
+--   | Term.bool b => sorry
+
+-- TODO: for a discrete order on α, WfD unique, Wf ==> WfD
+
+-- TODO: FWfD, FWf, associated lore
+
+-- TODO: propositional variants for below...
+
+inductive Body.WfD : Ctx α ε → Body φ → Ctx α ε → Type _
+  | nil : WfD Γ nil []
+  | let1 : a.WfD Γ A e → b.WfD (⟨A, e⟩::Γ) Δ → (let1 a b).WfD Γ (⟨A, e⟩::Δ)
+  | let2 : a.WfD Γ (Ty.pair A B) e
+    → b.WfD (⟨A, e⟩::⟨B, e⟩::Γ) Δ
+    → (let2 a b).WfD Γ (⟨A, e⟩::⟨B, e⟩::Δ)
+
+def LCtx (α) := List (Ty α)
+
+structure LCtx.Trg (L : LCtx α) (n : ℕ) (A : Ty α) : Prop where
+  length : n < L.length
+  get : A ≤ L.get ⟨n, length⟩
+
+instance : Append (LCtx α) := (inferInstance : Append (List (Ty α)))
+
+def FLCtx (α) := Σn, Fin n → Ty α
+
+-- TODO: FLCtx append
+
+inductive Terminator.WfD : Ctx α ε → Terminator φ → LCtx α → Type _
+  | br : L.Trg n A → a.WfD Γ A 0 → WfD Γ (br n a) L
+  | ite : e.WfD Γ Ty.bool 0 → s.WfD Γ L → t.WfD Γ L → WfD Γ (ite e s t) L
+
+structure Block.WfD (Γ : Ctx α ε) (β : Block φ) (Δ : Ctx α ε) (L : LCtx α) where
+  body : β.body.WfD Γ Δ
+  terminator : β.terminator.WfD (Δ ++ Γ) L
+
+inductive BBRegion.WfD : Ctx α ε → BBRegion φ → LCtx α → Type _
+  | cfg {Δ} : β.WfD Γ Δ K → (∀i : Fin n, (G i).WfD (Δ ++ Γ) K)
+    → L = K.drop n → BBRegion.WfD Γ (cfg β n G) L
+
+inductive TRegion.WfD : Ctx α ε → TRegion φ → LCtx α → Type _
+  | let1 : a.WfD Γ A e → t.WfD (⟨A, e⟩::Γ) L → (let1 a t).WfD Γ L
+  | let2 : a.WfD Γ (Ty.pair A B) e → t.WfD (⟨A, e⟩::⟨B, e⟩::Γ) L → (let2 a t).WfD Γ L
+  | cfg : t.WfD Γ K → (∀i : Fin n, (G i).WfD Γ K) → L = K.drop n → WfD Γ (cfg t n G) L
+
+inductive Region.WfD : Ctx α ε → Region φ → LCtx α → Type _
+  | br : L.Trg n A → a.WfD Γ A 0 → WfD Γ (br n a) L
+  | ite : e.WfD Γ Ty.bool 0 → s.WfD Γ L → t.WfD Γ L → WfD Γ (ite e s t) L
+  | let1 : a.WfD Γ A e → t.WfD (⟨A, e⟩::Γ) L → (let1 a t).WfD Γ L
+  | let2 : a.WfD Γ (Ty.pair A B) e → t.WfD (⟨A, e⟩::⟨B, e⟩::Γ) L → (let2 a t).WfD Γ L
+  | cfg : β.WfD Γ K → (∀i : Fin n, (G i).WfD Γ K) → L = K.drop n → WfD Γ (cfg β n G) L
+
+-- TODO: normalize region to TRegion; type preservation
+
+-- TODO: normalize TRegion to BBRegion; type preservation
+
+end Basic
+
+section Weakening
+
+variable
+  [Φ: InstSet φ (Ty α) ε] [PartialOrder α] [PartialOrder ε] [Zero ε]
+  {Γ Δ : Ctx α ε} {ρ : ℕ → ℕ} -- {a b : Term φ} {A B : Ty α} {e e' : ε}
+
 def Ctx.Wkn (Γ Δ : Ctx α ε) (ρ : ℕ → ℕ) : Prop -- TODO: fin argument as defeq?
   := ∀i, (h : i < Δ.length) → Γ.Var (ρ i) (Δ.get ⟨i, h⟩)
 
@@ -65,52 +168,25 @@ theorem Ctx.Wkn_def' (Γ Δ : Ctx α ε) (ρ : ℕ → ℕ) : Γ.Wkn Δ ρ ↔
 theorem Ctx.Wkn_iff (Γ Δ : Ctx α ε) (ρ : ℕ → ℕ) : Γ.Wkn Δ ρ ↔ List.NWkn Γ Δ ρ
   := ⟨λh i hi => have h' := h i hi; ⟨h'.length, h'.get⟩, λh i hi => have h' := h i hi; ⟨h'.1, h'.2⟩⟩
 
-theorem Ctx.Var.wk_res {Γ : Ctx α ε} {n : ℕ} {V V'} (h : V ≤ V') (hΓ : Γ.Var n V) : Γ.Var n V' where
+theorem Ctx.Var.wk_res (h : V ≤ V') (hΓ : Γ.Var n V) : Γ.Var n V' where
   length := hΓ.length
   get := le_trans hΓ.get h
 
-theorem Ctx.Var.wk_res₂ {Γ : Ctx α ε} {n : ℕ} {A A'} {e e'} (hA : A ≤ A') (he : e ≤ e')
-  (hΓ : Γ.Var n ⟨A, e⟩) : Γ.Var n ⟨A', e⟩ := hΓ.wk_res (by simp [hA, he])
+theorem Ctx.Var.wk_res₂ (hA : A ≤ A') (he : e ≤ e') (hΓ : Γ.Var n ⟨A, e⟩) : Γ.Var n ⟨A', e⟩
+  := hΓ.wk_res (by simp [hA, he])
 
-theorem Ctx.Var.wk_ty {Γ : Ctx α ε} {n : ℕ} {A A'} {e} (h : A ≤ A')
-  (hΓ : Γ.Var n ⟨A, e⟩) : Γ.Var n ⟨A', e⟩ := hΓ.wk_res (by simp [h])
+theorem Ctx.Var.wk_ty (h : A ≤ A') (hΓ : Γ.Var n ⟨A, e⟩) : Γ.Var n ⟨A', e⟩
+  := hΓ.wk_res (by simp [h])
 
-theorem Ctx.Var.wk_eff {Γ : Ctx α ε} {n : ℕ} {A} {e e'} (h : e ≤ e')
-  (hΓ : Γ.Var n ⟨A, e⟩) : Γ.Var n ⟨A, e'⟩ := hΓ.wk_res (by simp [h])
+theorem Ctx.Var.wk_eff (h : e ≤ e') (hΓ : Γ.Var n ⟨A, e⟩) : Γ.Var n ⟨A, e'⟩
+  := hΓ.wk_res (by simp [h])
 
-theorem Ctx.Var.wk
-  {Γ : Ctx α ε} {n : ℕ} {A : Ty α} {e : ε}
-  {Δ : Ctx α ε} {ρ : ℕ → ℕ} (h : Γ.Wkn Δ ρ) (hΓ : Δ.Var n ⟨A, e⟩) : Γ.Var (ρ n) ⟨A, e⟩ where
+theorem Ctx.Var.wk (h : Γ.Wkn Δ ρ) (hΓ : Δ.Var n ⟨A, e⟩) : Γ.Var (ρ n) ⟨A, e⟩ where
   length := (h n hΓ.length).1
   get := le_trans (h n hΓ.length).2 hΓ.get
 
-instance : Append (Ctx α ε) := (inferInstance : Append (List (Ty α × ε)))
-
-def FCtx (α ε) := Σn, Fin n → Ty α × ε
-
--- TODO: FCtx append
-
-inductive Term.Wf : Ctx α ε → Term φ → Ty α → ε → Prop
-| var {Γ n A e} : Γ.Var n ⟨A, e⟩ → Wf Γ (var n) A e
-| op {f : φ} {a e A B} : Φ.Fn f A B e → Wf Γ a A e → Wf Γ (op f a) B e
-| pair {a b A B e} : Wf Γ a A e → Wf Γ b B e → Wf Γ (pair a b) (Ty.pair A B) e
-| unit (e) : Wf Γ unit Ty.unit e
-| bool (b e) : Wf Γ (bool b) Ty.bool e
-
-inductive Term.WfD : Ctx α ε → Term φ → Ty α → ε → Type _
-| var : Γ.Var n ⟨A, e⟩ → WfD Γ (var n) A e
-| op : Φ.Fn f A B e → WfD Γ a A e → WfD Γ (op f a) B e
-| pair : WfD Γ a A e → WfD Γ b B e → WfD Γ (pair a b) (Ty.pair A B) e
-| unit (e) : WfD Γ unit Ty.unit e
-| bool (b e) : WfD Γ (bool b) Ty.bool e
-
--- TODO: WfD ==> Wf
-
--- TODO: Wf ==> ∃WfD
-
 /-- Weaken the effect of a term derivation -/
-def Term.WfD.wk_eff
-  {Γ : Ctx α ε} {a : Term φ} {A e} (h : e ≤ e') : WfD Γ a A e → WfD Γ a A e'
+def Term.WfD.wk_eff {a : Term φ} {A e} (h : e ≤ e') : WfD Γ a A e → WfD Γ a A e'
   | var dv => var (dv.wk_eff h)
   | op df de => op (df.wk_eff h) (de.wk_eff h)
   | pair dl dr => pair (dl.wk_eff h) (dr.wk_eff h)
@@ -118,24 +194,18 @@ def Term.WfD.wk_eff
   | bool b e => bool b e'
 
 /-- Weaken a term derivation -/
-def Term.WfD.wk
-  {Γ : Ctx α ε} {a : Term φ} {A e} {Δ : Ctx α ε} {ρ : ℕ → ℕ} (h : Γ.Wkn Δ ρ)
-  : WfD Δ a A e → WfD Γ (a.wk ρ) A e
+def Term.WfD.wk {a : Term φ} (h : Γ.Wkn Δ ρ) : WfD Δ a A e → WfD Γ (a.wk ρ) A e
   | var dv => var (dv.wk h)
   | op df de => op df (de.wk h)
   | pair dl dr => pair (dl.wk h) (dr.wk h)
   | unit e => unit e
   | bool b e => bool b e
 
--- TODO: for a discrete order on α, WfD unique, Wf ==> WfD
+-- TODO: Body:
 
--- TODO: FWfD, FWf, associated lore
+-- TODO: weakening
 
-def LCtx (α) := List (Ty α)
-
-structure LCtx.Trg (L : LCtx α) (n : ℕ) (A : Ty α) : Prop where
-  length : n < L.length
-  get : A ≤ L.get ⟨n, length⟩
+variable {L K : LCtx α}
 
 def LCtx.Wkn (L K : LCtx α) (ρ : ℕ → ℕ) : Prop -- TODO: fin argument as defeq?
   := ∀i, (h : i < L.length) → K.Trg (ρ i) (L.get ⟨i, h⟩)
@@ -149,75 +219,62 @@ theorem LCtx.Wkn_def' (L K : LCtx α) (ρ : ℕ → ℕ) : L.Wkn K ρ ↔
 theorem LCtx.Wkn_iff (L K : LCtx α) (ρ : ℕ → ℕ) : L.Wkn K ρ ↔ @List.NWkn (Ty α)ᵒᵈ _ K L ρ
   := ⟨λh i hi => have h' := h i hi; ⟨h'.length, h'.get⟩, λh i hi => have h' := h i hi; ⟨h'.1, h'.2⟩⟩
 
-theorem LCtx.Trg.wk
-  {L : LCtx α} {n : ℕ} {A : Ty α}
-  {K : LCtx α} {ρ : ℕ → ℕ} (h : L.Wkn K ρ) (hK : L.Trg n A) : K.Trg (ρ n) A where
+theorem LCtx.Trg.wk (h : L.Wkn K ρ) (hK : L.Trg n A) : K.Trg (ρ n) A where
   length := (h n hK.length).1
   get := le_trans hK.get (h n hK.length).2
 
-instance : Append (LCtx α) := (inferInstance : Append (List (Ty α)))
-
-def FLCtx (α) := Σn, Fin n → Ty α
-
--- TODO: FLCtx append
-
-inductive Terminator.WfD : Ctx α ε → Terminator φ → LCtx α → Type _
-  | br : L.Trg n A → a.WfD Γ A 0 → WfD Γ (br n a) L
-  | ite : e.WfD Γ Ty.bool 0 → s.WfD Γ L → t.WfD Γ L → WfD Γ (ite e s t) L
+-- TODO: Terminator:
 
 -- TODO: weakening
 
 -- TODO: label-weakening
 
-inductive Body.WfD : Ctx α ε → Body φ → Ctx α ε → Type _
-  | nil : WfD Γ nil []
-  | let1 : a.WfD Γ A e → b.WfD (⟨A, e⟩::Γ) Δ → (let1 a b).WfD Γ (⟨A, e⟩::Δ)
-  | let2 : a.WfD Γ (Ty.pair A B) e
-    → b.WfD (⟨A, e⟩::⟨B, e⟩::Γ) Δ
-    → (let2 a b).WfD Γ (⟨A, e⟩::⟨B, e⟩::Δ)
-
--- TODO: weakening
-
-structure Block.WfD (Γ : Ctx α ε) (β : Block φ) (Δ : Ctx α ε) (L : LCtx α) where
-  body : β.body.WfD Γ Δ
-  terminator : β.terminator.WfD (Δ ++ Γ) L
+-- TODO: Block:
 
 -- TODO: weakening
 
 -- TODO: label-weakening
 
-inductive BBRegion.WfD : Ctx α ε → BBRegion φ → LCtx α → Type _
-  | cfg {Δ} : β.WfD Γ Δ K → (∀i : Fin n, (G i).WfD (Δ ++ Γ) K)
-    → L = K.drop n → BBRegion.WfD Γ (cfg β n G) L
+-- TODO: BBRegion:
 
 -- TODO: weakening
 
 -- TODO: label-weakening
 
-inductive TRegion.WfD : Ctx α ε → TRegion φ → LCtx α → Type _
-  | let1 : a.WfD Γ A e → t.WfD (⟨A, e⟩::Γ) L → (let1 a t).WfD Γ L
-  | let2 : a.WfD Γ (Ty.pair A B) e → t.WfD (⟨A, e⟩::⟨B, e⟩::Γ) L → (let2 a t).WfD Γ L
-  | cfg : t.WfD Γ K → (∀i : Fin n, (G i).WfD Γ K) → L = K.drop n → WfD Γ (cfg t n G) L
+-- TODO: TRegion:
 
 -- TODO: weakening
 
 -- TODO: label-weakening
 
-inductive Region.WfD [Φ: InstSet φ (Ty α) ε] [PartialOrder α] [PartialOrder ε] [Zero ε]
-    : Ctx α ε → Region φ → LCtx α → Type _
-  | br : L.Trg n A → a.WfD Γ A 0 → WfD Γ (br n a) L
-  | ite : e.WfD Γ Ty.bool 0 → s.WfD Γ L → t.WfD Γ L → WfD Γ (ite e s t) L
-  | let1 : a.WfD Γ A e → t.WfD (⟨A, e⟩::Γ) L → (let1 a t).WfD Γ L
-  | let2 : a.WfD Γ (Ty.pair A B) e → t.WfD (⟨A, e⟩::⟨B, e⟩::Γ) L → (let2 a t).WfD Γ L
-  | cfg : β.WfD Γ K → (∀i : Fin n, (G i).WfD Γ K) → L = K.drop n → WfD Γ (cfg β n G) L
+-- TODO: Region:
 
 -- TODO: weakening
 
 -- TODO: label-weakening
 
--- TODO: normalize region to TRegion; type preservation
+end Weakening
 
--- TODO: normalize TRegion to BBRegion; type preservation
+section Minimal
+
+variable [Φ: InstSet φ (Ty α) ε] [PartialOrder α] [SemilatticeSup ε] [OrderBot ε] [Zero ε]
+
+def Term.min_effect (Γ : Ctx α ε) : Term φ → ε
+  | var n => if h : n < Γ.length then (Γ.get ⟨n, h⟩).2 else 0
+  | op f _ => Φ.effect f
+  | pair a b => a.min_effect Γ ⊔ b.min_effect Γ
+  | unit => ⊥
+  | bool _ => ⊥
+
+theorem Term.WfD.min_effect_le
+  {Γ : Ctx α ε} {a : Term φ} {A e} (h : WfD Γ a A e) : a.min_effect Γ ≤ e
+  := match h with
+  | var dv => by simp [min_effect, dv.length, dv.get.right]
+  | op df de => df.effect
+  | pair dl dr => sup_le_iff.mpr ⟨dl.min_effect_le, dr.min_effect_le⟩
+  | unit _ | bool _ _ => bot_le
+
+end Minimal
 
 -- == SPECULATIVE ==
 
